feat: cast_le

src/QL/FOL/Tait/semantics.lean
@@ -66,23 +66,32 @@ lemma models_iff : S ⊧ᵀ σ ↔ formula.val S fin.nil σ :=
 by simp[models, fin.nil]
 
 end sentence
-
+/-
 namespace uniform_subformula
 
 variables (S : Structure L) {n} {me : ℕ → S} {e : fin n → S}
 
-@[simp] def val (me : ℕ → S) : ∀ {n} (e : fin n → S), uniform_subformula L n → Prop
+@[simp] def val' (me : ℕ → S) : ∀ {n} (e : fin n → S), uniform_subformula L n → Prop
 | n _ verum              := true
 | n _ falsum             := false
 | n e (relation p v)     := S.pr p (uniform_subterm.val S me e ∘ v)
 | n e (neg_relation p v) := ¬S.pr p (uniform_subterm.val S me e ∘ v)
-| n e (and p q)          := p.val e ∧ q.val e
-| n e (or p q)           := p.val e ∨ q.val e
-| n e (fal p)            := ∀ x : S, (p.val (x *> e))
-| n e (ex p)             := ∃ x : S, (p.val (x *> e))
+| n e (and p q)          := p.val' e ∧ q.val' e
+| n e (or p q)           := p.val' e ∨ q.val' e
+| n e (fal p)            := ∀ x : S, (p.val' (x *> e))
+| n e (ex p)             := ∃ x : S, (p.val' (x *> e))
 
-@[simp] lemma val_neg (p : uniform_subformula L n) : val S me e (not p) = ¬val S me e p :=
-by induction p generalizing me e; simp[or_iff_not_imp_left, *]
+@[simp] lemma val'_neg (p : uniform_subformula L n) : val' S me e (∼p) = ¬val' S me e p :=
+by simp[←not_eq]; induction p generalizing me e; simp[or_iff_not_imp_left, *]
+
+@[irreducible] def val (me : ℕ → S) (e : fin n → S) : uniform_subformula L n →ₗ Prop :=
+{ to_fun := val' S me e,
+  map_neg' := λ _, by simp,
+  map_imply' := λ _ _, by simp[imply_def, or_iff_not_imp_left, ←or_eq],
+  map_and' := λ p q, by unfold has_inf.inf; simp; refl,
+  map_or' := λ p q, by unfold has_sup.sup; simp; refl,
+  map_top' := by refl,
+  map_bot' := by refl }
 
 @[simp] lemma val_relation {p} (r : L.pr p) (v) :
   val S me e (relation r v) ↔ S.pr r (uniform_subterm.val S me e ∘ v) :=  by simp[val]; refl
@@ -91,33 +100,46 @@ by induction p generalizing me e; simp[or_iff_not_imp_left, *]
   val S me e (neg_relation r v) ↔ ¬S.pr r (uniform_subterm.val S me e ∘ v) := by simp[val]; refl
 
 @[simp] lemma val_fal (p : uniform_subformula L (n + 1)) :
-  val S me e (fal p) ↔ ∀ x : S, val S me (x *> e) p := by simp[val]; refl
+  val S me e (∀'p) ↔ ∀ x : S, val S me (x *> e) p := by simp[val]; refl
 
 @[simp] lemma val_ex (p : uniform_subformula L (n + 1)) :
-  val S me e (ex p) ↔ ∃ x : S, val S me (x *> e) p := by simp[val]; refl
+  val S me e (∃'p) ↔ ∃ x : S, val S me (x *> e) p := by simp[val]; refl
 
 @[simp] lemma val_subst : ∀ {n} {e : fin n → S} (t : uniform_subterm L n) (p : uniform_subformula L (n + 1)),
   val S me e (subst t p) ↔ val S me (e <* t.val S me e) p
-| n e t verum := by simp
-| n e t falsum := by simp
-| n e t (relation r v) := by simp[(∘)]
+| n e t verum              := by simp[verum_eq]
+| n e t falsum             := by simp[falsum_eq]
+| n e t (relation r v)     := by simp[(∘)]
 | n e t (neg_relation r v) := by simp[(∘)]
-| n e t (and p q) := by simp[val_subst t p, val_subst t q]
-| n e t (or p q) := by simp[val_subst t p, val_subst t q]
-| n e t (fal p) := by simp[val_subst t.lift p, fin.left_right_concat_assoc]
-| n e t (ex p) := by simp[val_subst t.lift p, fin.left_right_concat_assoc]
+| n e t (and p q)          := by simp[and_eq, val_subst t p, val_subst t q]
+| n e t (or p q)           := by simp[or_eq, val_subst t p, val_subst t q]
+| n e t (fal p)            := by simp[fal_eq, val_subst t.lift p, fin.left_right_concat_assoc]
+| n e t (ex p)             := by simp[ex_eq, val_subst t.lift p, fin.left_right_concat_assoc]
 using_well_founded {rel_tac := λ _ _, `[exact ⟨_, measure_wf (λ x, x.2.2.2.complexity)⟩]}
 
 end uniform_subformula
+
+namespace uniform_formula
+variables (S : Structure L) {m n} (me : ℕ → S)
+
+def val : uniform_formula L →ₗ Prop := uniform_subformula.val S me fin.nil  
+
+end uniform_formula
+
+def uniform_models (S : Structure L) (p : uniform_formula L) : Prop := ∀ e, uniform_formula.val S e p
+
+infix (name := Tait.uniform_models) ` ⊧ᵀᵤ ` :55 := uniform_models
 
 namespace subformula
 variables (S : Structure L) {n} {me : ℕ → S} {e : fin n → S}
 
 lemma val_uniform (p : subformula L m n) : uniform_subformula.val S me e p.uniform ↔ val S (λ i, me i) e p :=
-by induction p; simp[verum_eq, falsum_eq, and_eq, or_eq, fal_eq, ex_eq, (∘), *]
+by { induction p; simp[verum_eq, uniform_subformula.verum_eq, falsum_eq, uniform_subformula.falsum_eq,
+     and_eq, uniform_subformula.and_eq, or_eq, uniform_subformula.or_eq, fal_eq, uniform_subformula.fal_eq,
+     ex_eq, uniform_subformula.ex_eq, (∘), *] }
 
 end subformula
-
+-/
 end Tait
 
 end fol
